Proof libs changes to lax-check TLS codec.

hax-lib/proof-libs/fstar/core/Core.Hash.fsti
@@ -1,5 +1,67 @@
 module Core.Hash
 
-class t_Hash (h: Type) = {
-  dummy_hash_field: unit
+
+open Rust_primitives.Arrays
+open Rust_primitives.Integers
+
+class t_Hasher (v_Self: Type0) = {
+  hax_dummy_hasher_field: Prims.unit;
 }
+
+class t_Hash (v_Self: Type0) = {
+  f_hash_pre:
+      #v_H: Type0 ->
+      {| i1: t_Hasher v_H |} ->
+      v_Self ->
+      v_H
+    -> Type0;
+  f_hash_post:
+      #v_H: Type0 ->
+      {| i1: t_Hasher v_H |} ->
+      v_Self ->
+      v_H ->
+      v_H
+    -> Type0;
+  f_hash:
+      #v_H: Type0 ->
+      {| i1: t_Hasher v_H |} ->
+      x0: v_Self ->
+      x1: v_H
+    -> Prims.Pure v_H
+        (f_hash_pre #v_H #i1 x0 x1)
+        (fun result ->
+            f_hash_post #v_H
+              #i1
+              x0
+              x1
+              result);
+  (* f_hash_slice_pre:
+      #v_H: Type0 ->
+      {| i1: t_Hasher v_H |} ->
+      t_Slice v_Self ->
+      v_H
+    -> Type0;
+  f_hash_slice_post:
+      #v_H: Type0 ->
+      {| i1: t_Hasher v_H |} ->
+      t_Slice v_Self ->
+      v_H ->
+      v_H
+    -> Type0;
+  f_hash_slice:
+      #v_H: Type0 ->
+      {| i1: t_Hasher v_H |} ->
+      x0: t_Slice v_Self ->
+      x1: v_H
+    -> Prims.Pure v_H
+        (f_hash_slice_pre #v_H #i1 x0 x1)
+        (fun result ->
+            f_hash_slice_post #v_H
+              #i1
+              x0
+              x1
+              result) *)
+}
+
+[@@ FStar.Tactics.Typeclasses.tcinstance]
+val hash_vec (t: Type0): t_Hash (Alloc.Vec.t_Vec t Alloc.Alloc.t_Global)
