hax-lib/proof-libs/fstar/core/Core.Fmt.Rt.fsti
@@ -7,9 +7,12 @@ val impl_1__new_debug (#t:Type0) (x: t): t_Argument
 val impl_4__new_v1_formatted (#t:Type0) (x: t) : t_Argument
 val impl_1__new_binary (#t:Type0) (x: t) : t_Argument
 val impl_1__new_lower_hex (#t:Type0) (x: t) : t_Argument
+val impl__new_lower_hex (#t:Type0) (x: t) : t_Argument
 val impl_1__new_const (#t:Type0) (#u:Type0) (xconst: t) (yconst: u): t_Argument
 val impl_1__new_v1 (#t1:Type0) (#t2:Type0) (#t3:Type0) (#t4:Type0) 
   (x1: t1) (x2: t2) (x3: t3) (x4: t4) : t_Argument
+val impl_1__new_v1_formatted (#t1:Type0) (#t2:Type0) (#t3:Type0) 
+  (x1: t1) (x2: t2) (x3: t3) : t_Argument
 val impl__new_display (#t:Type0) (x: t): t_Argument
 val impl__new_debug (#t:Type0) (x: t): t_Argument
 
@@ -20,8 +23,14 @@ type t_Count =
   | Count_Param : int_t U16 -> t_Count
   | Count_Implied : t_Count
 
-type t_Placeholder: Type0
+class t_Placeholder = {
+  f_position: usize;
+  f_flags: u32;
+  f_precision: t_Count;
+  f_width: t_Count
+}
 val impl_Placeholder__new : usize -> (int_t U32) -> t_Count -> t_Count -> t_Placeholder
 
 type t_UnsafeArg
 val impl_UnsafeArg__new : unit -> t_UnsafeArg
+
